src/Dafny/examples/fs/inode.dfy
@@ -1,0 +1,134 @@
+include "../../util/marshal.i.dfy"
+
+// NOTE: this module, unlike the others in this development, is not intended to
+// be opened
+module Inode {
+  import opened Machine
+  import IntEncoding
+  import opened Collections
+  import opened ByteSlice
+  import opened Marshal
+
+  datatype Inode = Mk(sz: uint64, blks: seq<uint64>)
+
+  function method div_roundup(x: nat, k: nat): nat
+    requires k >= 1
+  {
+    (x + (k-1)) / k
+  }
+
+  function method NextBlock(i:Inode): uint64
+  {
+    i.sz/4096
+  }
+
+  predicate Valid(i:Inode)
+  {
+    var blks_ := i.blks;
+    // only direct blocks
+    && |blks_| <= 15
+    // TODO: will be div_roundup
+    && |blks_| == i.sz as nat/4096
+    // TODO: generalize to allow non-block appends
+    && i.sz % 4096 == 0
+    && (forall bn | bn in blks_ :: bn != 0)
+    && unique(blks_)
+  }
+
+
+  function inode_enc(i: Inode): seq<Encodable>
+  {
+    [EncUInt64(i.sz)] + seq_fmap(blkno => EncUInt64(blkno), i.blks)
+  }
+
+  lemma {:induction xs} enc_uint64_len(xs: seq<uint64>)
+    ensures |seq_encode(seq_fmap(blkno => EncUInt64(blkno), xs))| == 8*|xs|
+  {}
+
+  function enc(i: Inode): (bs:seq<byte>)
+    requires Valid(i)
+    ensures |bs| == 128
+  {
+    enc_uint64_len(i.blks);
+    assert |seq_encode(inode_enc(i))| == 8+8*|i.blks|;
+    seq_encode(inode_enc(i)) + repeat(0 as byte, 128-(8+8*|i.blks|))
+  }
+
+  const zero: Inode := Mk(0, []);
+
+  lemma zero_valid()
+    ensures Valid(zero)
+  {}
+
+  lemma zero_encoding()
+    ensures Valid(zero)
+    ensures repeat(0 as byte, 128) == enc(zero)
+  {
+    zero_valid();
+    //assert inode_enc(zero) == [EncUInt64(0)];
+    //assert repeat(0 as byte, 8) == [0,0,0,0,0,0,0,0];
+    repeat_split(0 as byte, 128, 8, 128-8);
+    IntEncoding.lemma_enc_0();
+  }
+
+  method encode_ino(i: Inode) returns (bs:Bytes)
+    modifies {}
+    requires Valid(i)
+    ensures fresh(bs)
+    ensures bs.data == enc(i)
+    ensures |bs.data| == 128
+  {
+    var e := new Encoder(128);
+    e.PutInt(i.sz);
+    var num_blocks := i.sz/4096;
+    assert num_blocks as nat == |i.blks|;
+    var k: uint64 := 0;
+    while k < num_blocks
+      modifies e.Repr
+      invariant e.Valid()
+      invariant 0 <= k <= num_blocks
+      invariant e.bytes_left() == 128 - ((k as nat+1)*8)
+      invariant e.enc ==
+      [EncUInt64(i.sz)] +
+      seq_fmap(blkno => EncUInt64(blkno), i.blks[..k])
+    {
+      e.PutInt(i.blks[k]);
+      k := k + 1;
+    }
+    assert i.blks[..|i.blks|] == i.blks;
+    assert e.enc == inode_enc(i);
+    bs := e.Finish();
+  }
+
+  method decode_ino(bs: Bytes, ghost i: Inode) returns (i': Inode)
+    modifies {}
+    requires bs.Valid()
+    requires Valid(i)
+    requires bs.data == enc(i)
+    ensures i' == i
+  {
+    var dec := new Decoder();
+    dec.Init(bs, inode_enc(i));
+    var sz := dec.GetInt(i.sz);
+    var num_blks := sz/4096;
+    assert num_blks as nat == |i.blks|;
+    assert dec.enc == seq_fmap(blkno => EncUInt64(blkno), i.blks);
+
+    var blks: seq<uint64> := [];
+
+    var k: uint64 := 0;
+    while k < num_blks
+      modifies dec
+      invariant dec.Valid()
+      invariant Valid(i)
+      invariant 0 <= k <= num_blks
+      invariant blks == i.blks[..k]
+      invariant dec.enc == seq_fmap(blkno => EncUInt64(blkno), i.blks[k..])
+    {
+      var blk := dec.GetInt(i.blks[k]);
+      blks := blks + [blk];
+      k := k + 1;
+    }
+    return Mk(sz, blks);
+  }
+}
